SPos.lean
@@ -3,6 +3,7 @@ import SPos.SyntaxProperties
 
 import SPos.Typing.WellTyped
 
+import SPos.Semantics.PER
 import SPos.Semantics.Domain
 import SPos.Semantics.ValueDomain
 import SPos.Semantics.Eval
