SPos/Semantics/PER.lean
@@ -1,0 +1,19 @@
+
+structure PER (D : Type u) where
+  R     : D → D → Prop
+  symm  : Symm R
+  trans : Transitive R
+
+namespace IsPER
+
+variable {D : Type u} {R : D → D → Prop}
+
+/-- Anything related is in the domain (self-related), on the left. -/
+theorem refl_left (h : IsPER R) {a b : D} (hab : R a b) : R a a :=
+  h.trans hab (h.symm hab)
+
+/-- Anything related is in the domain (self-related), on the right. -/
+theorem refl_right (h : IsPER R) {a b : D} (hab : R a b) : R b b :=
+  h.trans (h.symm hab) hab
+
+end IsPER
